hax-lib/proof-libs/fstar/core/Core_models.Cmp.fst
@@ -99,126 +99,126 @@ include Core_models.Bundle {impl_4 as impl_4}
 
 include Core_models.Bundle {impl_5__from__cmp as impl_5}
 
-include Core_models.Bundle {impl_6 as impl_6}
+include Core_models.Bundle {impl_34 as impl_34}
 
-include Core_models.Bundle {impl_7__from__cmp as impl_Ord_for_u8}
-
-include Core_models.Bundle {impl_8 as impl_8}
-
-include Core_models.Bundle {impl_9 as impl_Eq_for_u8}
+include Core_models.Bundle {impl_35__from__cmp as impl_Ord_for_u8}
 
 include Core_models.Bundle {impl_10 as impl_10}
 
-include Core_models.Bundle {impl_11__from__cmp as impl_Ord_for_i8}
+include Core_models.Bundle {impl_11 as impl_Eq_for_u8}
+
+include Core_models.Bundle {impl_36 as impl_36}
+
+include Core_models.Bundle {impl_37__from__cmp as impl_Ord_for_i8}
 
 include Core_models.Bundle {impl_12 as impl_12}
 
 include Core_models.Bundle {impl_13 as impl_Eq_for_i8}
 
-include Core_models.Bundle {impl_14 as impl_14}
-
-include Core_models.Bundle {impl_15__from__cmp as impl_Ord_for_u16}
-
-include Core_models.Bundle {impl_16 as impl_16}
-
-include Core_models.Bundle {impl_17 as impl_Eq_for_u16}
-
-include Core_models.Bundle {impl_18 as impl_18}
-
-include Core_models.Bundle {impl_19__from__cmp as impl_Ord_for_i16}
-
-include Core_models.Bundle {impl_20 as impl_20}
-
-include Core_models.Bundle {impl_21 as impl_Eq_for_i16}
-
-include Core_models.Bundle {impl_22 as impl_22}
-
-include Core_models.Bundle {impl_23__from__cmp as impl_Ord_for_u32}
-
-include Core_models.Bundle {impl_24__from__cmp as impl_24}
-
-include Core_models.Bundle {impl_25__from__cmp as impl_Eq_for_u32}
-
-include Core_models.Bundle {impl_26__from__cmp as impl_26}
-
-include Core_models.Bundle {impl_27__from__cmp as impl_Ord_for_i32}
-
-include Core_models.Bundle {impl_28__from__cmp as impl_28}
-
-include Core_models.Bundle {impl_29__from__cmp as impl_Eq_for_i32}
-
-include Core_models.Bundle {impl_30__from__cmp as impl_30}
-
-include Core_models.Bundle {impl_31__from__cmp as impl_Ord_for_u64}
-
-include Core_models.Bundle {impl_32 as impl_32}
-
-include Core_models.Bundle {impl_33 as impl_Eq_for_u64}
-
-include Core_models.Bundle {impl_34 as impl_34}
-
-include Core_models.Bundle {impl_35__from__cmp as impl_Ord_for_i64}
-
-include Core_models.Bundle {impl_36 as impl_36}
-
-include Core_models.Bundle {impl_37 as impl_Eq_for_i64}
-
 include Core_models.Bundle {impl_38 as impl_38}
 
-include Core_models.Bundle {impl_39__from__cmp as impl_Ord_for_u128}
+include Core_models.Bundle {impl_39__from__cmp as impl_Ord_for_u16}
+
+include Core_models.Bundle {impl_14 as impl_14}
+
+include Core_models.Bundle {impl_15 as impl_Eq_for_u16}
 
 include Core_models.Bundle {impl_40 as impl_40}
 
-include Core_models.Bundle {impl_41 as impl_Eq_for_u128}
+include Core_models.Bundle {impl_41__from__cmp as impl_Ord_for_i16}
+
+include Core_models.Bundle {impl_16 as impl_16}
+
+include Core_models.Bundle {impl_17 as impl_Eq_for_i16}
 
 include Core_models.Bundle {impl_42 as impl_42}
 
-include Core_models.Bundle {impl_43__from__cmp as impl_Ord_for_i128}
+include Core_models.Bundle {impl_43__from__cmp as impl_Ord_for_u32}
+
+include Core_models.Bundle {impl_18 as impl_18}
+
+include Core_models.Bundle {impl_19 as impl_Eq_for_u32}
 
 include Core_models.Bundle {impl_44 as impl_44}
 
-include Core_models.Bundle {impl_45 as impl_Eq_for_i128}
+include Core_models.Bundle {impl_45__from__cmp as impl_Ord_for_i32}
+
+include Core_models.Bundle {impl_20 as impl_20}
+
+include Core_models.Bundle {impl_21 as impl_Eq_for_i32}
 
 include Core_models.Bundle {impl_46 as impl_46}
 
-include Core_models.Bundle {impl_47__from__cmp as impl_Ord_for_usize}
+include Core_models.Bundle {impl_47__from__cmp as impl_Ord_for_u64}
+
+include Core_models.Bundle {impl_22 as impl_22}
+
+include Core_models.Bundle {impl_23 as impl_Eq_for_u64}
 
 include Core_models.Bundle {impl_48 as impl_48}
 
-include Core_models.Bundle {impl_49 as impl_Eq_for_usize}
+include Core_models.Bundle {impl_49__from__cmp as impl_Ord_for_i64}
+
+include Core_models.Bundle {impl_24__from__cmp as impl_24}
+
+include Core_models.Bundle {impl_25__from__cmp as impl_Eq_for_i64}
 
 include Core_models.Bundle {impl_50 as impl_50}
 
-include Core_models.Bundle {impl_51__from__cmp as impl_Ord_for_isize}
+include Core_models.Bundle {impl_51__from__cmp as impl_Ord_for_u128}
+
+include Core_models.Bundle {impl_26__from__cmp as impl_26}
+
+include Core_models.Bundle {impl_27__from__cmp as impl_Eq_for_u128}
 
 include Core_models.Bundle {impl_52 as impl_52}
 
-include Core_models.Bundle {impl_53 as impl_Eq_for_isize}
+include Core_models.Bundle {impl_53__from__cmp as impl_Ord_for_i128}
 
-include Core_models.Bundle {impl_54__is_eq as impl_Ordering__is_eq}
+include Core_models.Bundle {impl_28__from__cmp as impl_28}
 
-include Core_models.Bundle {impl_54__is_ne as impl_Ordering__is_ne}
+include Core_models.Bundle {impl_29__from__cmp as impl_Eq_for_i128}
 
-include Core_models.Bundle {impl_54__is_lt as impl_Ordering__is_lt}
+include Core_models.Bundle {impl_54 as impl_54}
 
-include Core_models.Bundle {impl_54__is_gt as impl_Ordering__is_gt}
+include Core_models.Bundle {impl_55__from__cmp as impl_Ord_for_usize}
 
-include Core_models.Bundle {impl_54__is_le as impl_Ordering__is_le}
+include Core_models.Bundle {impl_30__from__cmp as impl_30}
 
-include Core_models.Bundle {impl_54__is_ge as impl_Ordering__is_ge}
+include Core_models.Bundle {impl_31__from__cmp as impl_Eq_for_usize}
 
-include Core_models.Bundle {impl_54__reverse as impl_Ordering__reverse}
+include Core_models.Bundle {impl_56 as impl_56}
 
-include Core_models.Bundle {impl_54__then as impl_Ordering__then}
+include Core_models.Bundle {impl_57__from__cmp as impl_Ord_for_isize}
 
-include Core_models.Bundle {impl_54__then_with as impl_Ordering__then_with}
+include Core_models.Bundle {impl_32 as impl_32}
+
+include Core_models.Bundle {impl_33 as impl_Eq_for_isize}
+
+include Core_models.Bundle {impl_58__is_eq as impl_Ordering__is_eq}
+
+include Core_models.Bundle {impl_58__is_ne as impl_Ordering__is_ne}
+
+include Core_models.Bundle {impl_58__is_lt as impl_Ordering__is_lt}
+
+include Core_models.Bundle {impl_58__is_gt as impl_Ordering__is_gt}
+
+include Core_models.Bundle {impl_58__is_le as impl_Ordering__is_le}
+
+include Core_models.Bundle {impl_58__is_ge as impl_Ordering__is_ge}
+
+include Core_models.Bundle {impl_58__reverse as impl_Ordering__reverse}
+
+include Core_models.Bundle {impl_58__then as impl_Ordering__then}
+
+include Core_models.Bundle {impl_58__then_with as impl_Ordering__then_with}
 
 include Core_models.Bundle {clamp as clamp}
 
-include Core_models.Bundle {impl_55 as impl_55}
+include Core_models.Bundle {impl_6 as impl_6}
 
-include Core_models.Bundle {impl_56 as impl_Eq_for_tuple_}
+include Core_models.Bundle {impl_7 as impl_Eq_for_tuple_}
 
-include Core_models.Bundle {impl_57 as impl_57}
+include Core_models.Bundle {impl_8 as impl_8}
 
-include Core_models.Bundle {impl_58__from__cmp as impl_Ord_for_tuple_}
+include Core_models.Bundle {impl_9__from__cmp as impl_Ord_for_tuple_}
