hax-lib/proof-libs/lean/CoreModels/Alloc/Types.lean
@@ -50,41 +50,41 @@ structure borrow.ToOwned (Self : Type) where
 def boxed.Box (T : Type) := T
 
 /-- [alloc::collections::btree::set::BTreeSet]
-    Source: 'src/lib.rs', lines 289:12-289:56 -/
+    Source: 'src/lib.rs', lines 287:12-287:56 -/
 def collections.btree.set.BTreeSet (T : Type) (U : Type) :=
   core.option.Option T × core.option.Option U
 
 /-- [alloc::collections::vec_deque::VecDeque]
-    Source: 'src/lib.rs', lines 317:8-317:75
+    Source: 'src/lib.rs', lines 315:8-315:75
     Visibility: public -/
 def collections.vec_deque.VecDeque (T : Type) (A : Type) :=
   rust_primitives.sequence.Seq T × core.marker.PhantomData A
 
 /-- [alloc::collections::vec_deque::into_iter::IntoIter]
-    Source: 'src/lib.rs', lines 362:12-362:83
+    Source: 'src/lib.rs', lines 360:12-360:83
     Visibility: public -/
 def collections.vec_deque.into_iter.IntoIter (T : Type) (A : Type) :=
   rust_primitives.sequence.Seq T × core.marker.PhantomData A
 
 /-- [alloc::slice::Dummy]
-    Source: 'src/lib.rs', lines 521:4-521:23 -/
+    Source: 'src/lib.rs', lines 519:4-519:23 -/
 @[reducible]
 def slice.Dummy (T : Type) := T
 
 /-- [alloc::vec::Vec]
-    Source: 'src/lib.rs', lines 737:4-737:34
+    Source: 'src/lib.rs', lines 735:4-735:34
     Visibility: public -/
 @[reducible]
 def vec.Vec (T : Type) := rust_primitives.sequence.Seq T
 
 /-- [alloc::vec::into_iter::IntoIter]
-    Source: 'src/lib.rs', lines 787:8-787:43
+    Source: 'src/lib.rs', lines 785:8-785:43
     Visibility: public -/
 @[reducible]
 def vec.into_iter.IntoIter (T : Type) := rust_primitives.sequence.Seq T
 
 /-- [alloc::vec::drain::Drain]
-    Source: 'src/lib.rs', lines 927:8-927:76
+    Source: 'src/lib.rs', lines 925:8-925:76
     Visibility: public -/
 def vec.drain.Drain (T : Type) (A : Type) :=
   rust_primitives.sequence.Seq T × core.marker.PhantomData A
